1) added attributes of callsite parameters to Vellvm, w/o them llvm-ld may generate wrong code.    output the datalayout config, w/o the config, llvm-ld can also go wrong.    We did not find the problem before because we run other LLVM optimizations after the SoftBound instrumentation, these LLVM passes somehow can fix the issues at some cases. But, if we do not run any opt, and llvm-ld the output with -disable-opt, the problem happens.
2)  all cases in olden-ccured are working (except bh, LLVM 2.6-gcc
cannot compile it).
   129.compress is also working
   But there are no observable performance difference between the
following configs.
   suppose in.bc is the original

   llvm with our GVN: 
      coqgvn in.bc >& out.bc
      llvm-ld out.bc -disable-opt -o test1.exe

   llvm with our GVN:
      llvm-ld in.bc -disable-opt -gvn -o test2.exe

   llvm without any GVN
      llvm-ld in.bc -disable-opt -o test3.exe

   These may not be the correct flags...

3) The function @findbestextension in 099.go is very slow to compile.
In the function there are 176 blocks, which compose of a 6-level
dom-tree.

    130.li and 132.jpeg crash for unknown problems.




git-svn-id: https://webdav.seas.upenn.edu/svn/sol/vol@3371 eef5ea85-cc2e-0410-bd84-0fae1f012da8

src/SoftBound/sb_def.v
@@ -2,6 +2,7 @@ Add LoadPath "../Vellvm/ott".
 Add LoadPath "../Vellvm/monads".
 Add LoadPath "../Vellvm".
 Add LoadPath "../Vellvm/compcert".
+Add LoadPath "../Vellvm/GraphBasics".
 Add LoadPath "../../../theory/metatheory_8.3".
 Add LoadPath "../TV".
 Require Import vellvm.
@@ -266,7 +267,7 @@ Fixpoint params2GVs (TD:TargetData) (lp:params) (lc:GVsMap) (gl:GVMap)
   (rm:rmetadata) : option (list (GVs * option metadata)) :=
 match lp with
 | nil => Some nil
-| (t, v)::lp' => 
+| ((t,_), v)::lp' => 
     match (getOperandValue TD v lc gl, params2GVs TD lp' lc gl rm) with
     | (Some gv, Some gvs) =>
        if isPointerTypB t then 
@@ -683,7 +684,7 @@ Tactic Notation "sb_sInsn_cases" tactic(first) tactic(c) :=
 (*
 *** Local Variables: ***
 *** coq-prog-name: "coqtop" ***
-*** coq-prog-args: ("-emacs-U" "-I" "~/SVN/sol/vol/src/Vellvm/monads" "-I" "~/SVN/sol/vol/src/Vellvm/ott" "-I" "~/SVN/sol/vol/src/Vellvm/compcert" "-I" "~/SVN/sol/theory/metatheory_8.3" "-I" "~/SVN/sol/vol/src/TV") ***
+*** coq-prog-args: ("-emacs-U" "-I" "~/SVN/sol/vol/src/Vellvm/monads" "-I" "~/SVN/sol/vol/src/Vellvm/ott" "-I" "~/SVN/sol/vol/src/Vellvm/compcert" "-I" "~/SVN/sol/theory/metatheory_8.3" "-I" "~/SVN/sol/vol/src/TV" "-impredicative-set") ***
 *** End: ***
  *)
 
