src/TV/sub_tv.v
@@ -2,6 +2,7 @@ Add LoadPath "../Vellvm/ott".
 Add LoadPath "../Vellvm/monads".
 Add LoadPath "../Vellvm".
 Add LoadPath "../Vellvm/compcert".
+Add LoadPath "../Vellvm/GraphBasics".
 Add LoadPath "../../../theory/metatheory_8.3".
 Require Import syntax.
 Require Import infrastructure.
@@ -348,17 +349,19 @@ Definition sub_sstate Ps1 Ps2 fid s1 s2 :=
 Definition tv_cmds Ps1 Ps2 fid (nbs1 nbs2 : list nbranch) :=
 sub_sstate Ps1 Ps2 fid (se_cmds sstate_init nbs1) (se_cmds sstate_init nbs2).
 
-Fixpoint tv_sparams Ps1 Ps2 fid (tsts1 tsts2:list (typ*sterm)) : bool :=
+Fixpoint tv_sparams Ps1 Ps2 fid (tsts1 tsts2:list (typ*attributes*sterm)) 
+  : bool :=
 match (tsts1, tsts2) with
 | (nil, _) => true
-| ((t1,st1)::tsts1', (t2,st2)::tsts2') => 
+| ((t1,_,st1)::tsts1', (t2,_,st2)::tsts2') => 
   tv_typ t1 t2 && tv_sterm Ps1 Ps2 fid st1 st2 && 
   tv_sparams Ps1 Ps2 fid tsts1' tsts2'
 | _ => false
 end.
 
 Inductive scall : Set :=
-| stmn_call : id -> noret -> clattrs -> typ -> sterm -> list (typ*sterm) -> scall
+| stmn_call : id -> noret -> clattrs -> typ -> sterm -> 
+    list (typ*attributes*sterm) -> scall
 .
 
 Definition se_call : forall (st : sstate)(i:cmd)(iscall:isCall i = true), scall.
@@ -875,11 +878,11 @@ rsub_sstate Ps1 Ps2 fid r (se_cmds sstate_init nbs1) (se_cmds sstate_init nbs2).
  * FunTable. Since the LLVM IR takes function names as function pointers,
  * if a program does not assign them to be other variables, they should
  * be the same. *)
-Fixpoint rtv_sparams Ps1 Ps2 fid r (tsts1 tsts2:list (typ*sterm)) : 
+Fixpoint rtv_sparams Ps1 Ps2 fid r (tsts1 tsts2:list (typ*attributes*sterm)) : 
   option renaming :=
 match (tsts1, tsts2) with
 | (nil, _) => Some r
-| ((t1,st1)::tsts1', (t2,st2)::tsts2') => 
+| ((t1,_,st1)::tsts1', (t2,_,st2)::tsts2') => 
   if tv_typ t1 t2 then
     rtv_sterm Ps1 Ps2 fid r st1 st2 >>=
     fun r => rtv_sparams Ps1 Ps2 fid r tsts1' tsts2'
@@ -1756,6 +1759,6 @@ Tactic Notation "sumbool_subst" "in" hyp(H) :=
 (*
 *** Local Variables: ***
 *** coq-prog-name: "coqtop" ***
-*** coq-prog-args: ("-emacs-U" "-I" "~/SVN/sol/vol/src/Vellvm/monads" "-I" "~/SVN/sol/vol/src/Vellvm/ott" "-I" "~/SVN/sol/vol/src/Vellvm/compcert" "-I" "~/SVN/sol/theory/metatheory_8.3") ***
+*** coq-prog-args: ("-emacs-U" "-I" "~/SVN/sol/vol/src/Vellvm/monads" "-I" "~/SVN/sol/vol/src/Vellvm/ott" "-I" "~/SVN/sol/vol/src/Vellvm/compcert" "-I" "~/SVN/sol/theory/metatheory_8.3" "-impredicative-set") ***
 *** End: ***
  *)
