src/Transforms/test.sh
@@ -6,38 +6,35 @@ GVN=../_build/Transforms/main.d.byte
 BC_DIR=./testcases/
 OC_DIR=./testcases/olden-ccured/
 # bh: llvm-gcc fails.
-# perimeter tsp: GVN is slow.
-OC_CASES="bisort em3d health mst power treeadd"
+OC_CASES="bisort em3d health mst perimeter power treeadd tsp"
 S95_DIR=./testcases/spec95-ccured/
 # 129.compress has floats and functions named like "\01__soc95" and "@^0"
 # In 099.go 130.li 132.ijpeg there are 'switch'
 # ijpeg: undefined reference to `softbound__01___isoc99_sscanf'
 # 132.ijpeg is slow for SBpass
 #S95_CASES="129.compress 099.go 130.li 132.ijpeg"
-S95_CASES=""
-OPT_FLAG=
+S95_CASES="129.compress"
+OPT_FLAG="-disable-opt -functionattrs -globaldce -globalopt -globalsmodref-aa \
+	-inline -instcombine -internalize -jump-threading -licm -loopsimplify \
+	-mem2reg -memdep -scalarrepl -sccp -simplifycfg"    
 
 for name in ./testcases/*.ll; do 
   echo -e $name": \c"  
   llvm-as -f $name -o input.bc
-  llvm-ld -disable-opt input.bc -o test.exe
-  echo -e "before \c"; time ./test.exe
   $GVN input.bc
   $GVN input.bc >& output.ll
   llvm-as -f output.ll
-  llvm-ld -disable-opt output.bc -o test.exe
-  echo -e "after \c"; time ./test.exe
+  llvm-ld output.bc -o test.exe
+  time ./test.exe
 done;
 for dir in $DIRS; do
   for name in $dir/*.ll; do 
     echo -e $name": \c"  
     llvm-as -f $name -o input.bc
-    llvm-ld -disable-opt input.bc -o test.exe
-    echo -e "before \c"; time ./test.exe
     $GVN input.bc >& output.ll
     llvm-as -f output.ll
     llvm-ld -disable-opt output.bc -o test.exe
-    echo -e "after \c"; time ./test.exe
+    time ./test.exe
   done;
 done;
 rm -f input.* output.* test.exe test.exe.bc
@@ -46,9 +43,9 @@ for name in $OC_CASES; do
   echo -e $name": \c" ; 
   $GVN $OC_DIR$name"/test.bc" >& $name"o.ll"
   llvm-as -f $name"o.ll" -o $name"o.bc"
-  llvm-ld -disable-opt $name"o.bc" -o $name"a.exe"
-  llvm-ld -disable-opt -gvn $OC_DIR$name"/test.bc" -o $name"b.exe"
-  llvm-ld -disable-opt $OC_DIR$name"/test.bc" -o $name"c.exe"
+  llvm-ld -native -lm $OPT_FLAG $name"o.bc" -o $name"a.exe"
+  llvm-ld -native -lm $OPT_FLAG -gvn $OC_DIR$name"/test.bc" -o $name"b.exe"
+  llvm-ld -native -lm $OPT_FLAG $OC_DIR$name"/test.bc" -o $name"c.exe"
 done;
 #echo -e "bh b: \c"; time ./bhb.exe;
 #echo -e "bh a: \c"; time ./bha.exe;
@@ -65,26 +62,31 @@ echo -e "health c: \c"; time ./healthc.exe 8 250 1;
 echo -e "mst b: \c"; time ./mstb.exe 4000;
 echo -e "mst a: \c"; time ./msta.exe 4000;
 echo -e "mst c: \c"; time ./mstc.exe 4000;
-#echo -e "perimeter b: \c"; time ./perimeterb.exe 12 2000;
-#echo -e "perimeter a: \c"; time ./perimetera.exe 12 2000;
-#echo -e "perimeter c: \c"; time ./perimeterc.exe 12 2000;
+echo -e "perimeter b: \c"; time ./perimeterb.exe 12 2000;
+echo -e "perimeter a: \c"; time ./perimetera.exe 12 2000;
+echo -e "perimeter c: \c"; time ./perimeterc.exe 12 2000;
 echo -e "power b: \c"; time ./powerb.exe;
 echo -e "power a: \c"; time ./powera.exe;
 echo -e "power c: \c"; time ./powerc.exe;
 echo -e "treeadd b: \c"; time ./treeaddb.exe 24 10; 
 echo -e "treeadd a: \c"; time ./treeadda.exe 24 10; 
 echo -e "treeadd c: \c"; time ./treeaddc.exe 24 10; 
-#echo -e "tsp b: \c"; time ./tspb.exe 2000000 0;
-#echo -e "tsp a: \c"; time ./tspa.exe 2000000 0;
-#echo -e "tsp c: \c"; time ./tspc.exe 2000000 0;
+echo -e "tsp b: \c"; time ./tspb.exe 2000000 0;
+echo -e "tsp a: \c"; time ./tspa.exe 2000000 0;
+echo -e "tsp c: \c"; time ./tspc.exe 2000000 0;
 for name in $S95_CASES; do 
   echo -e $name": \c" ; 
   $GVN $S95_DIR$name"/src/test.bc" >& $name"o.ll"
   llvm-as -f $name"o.ll" -o $name"o.bc"
-  llvm-ld -disable-opt $name"o.bc" -o $name".exe"
+  llvm-ld -native -lm $OPT_FLAG $name"o.bc" -o $name"a.exe"
+  llvm-ld -native -lm $OPT_FLAG -gvn $S95_DIR$name"/src/test.bc" -o $name"b.exe"
+  llvm-ld -native -lm $OPT_FLAG $S95_DIR$name"/src/test.bc" -o $name"c.exe"
 done;
 #echo -e "099.go: \c"; time ./099.go.exe 100 15;
 #echo -e "130.li: \c"; time ./130.li.exe ./testcases/spec95-ccured/130.li/src/ref.lsp;
+#echo -e "129.compress b: \c"; time ./129.compressb.exe ./testcases/spec95-ccured/129.compress/src/slow_input.data
+#echo -e "129.compress a: \c"; time ./129.compressa.exe ./testcases/spec95-ccured/129.compress/src/slow_input.data
+#echo -e "129.compress c: \c"; time ./129.compressc.exe ./testcases/spec95-ccured/129.compress/src/slow_input.data
 rm -f bisort* em3d* health* mst* treeadd* 129.compress* test-softbound.bc \
   130.li* 099.go* tsp* bh* power* perimeter*
 
